Logic/Modal/Standard/Kripke/Soundness.lean
@@ -10,7 +10,7 @@ open Formula
 
 open DeductionParameter (Normal)
 
-lemma sound [definability : Ax.DefinesKripkeFrameClass 𝔽] (d : (Normal Ax) ⊢! p) : 𝔽 ⊧ p := by
+lemma sound [definability : Ax.DefinesKripkeFrameClass 𝔽] (d : Axᴺ ⊢! p) : 𝔽 ⊧ p := by
   induction d using Deduction.inducition_with_necOnly! with
   | hMaxm h =>
     simp only [Set.mem_setOf_eq] at h;
@@ -28,25 +28,56 @@ lemma sound [definability : Ax.DefinesKripkeFrameClass 𝔽] (d : (Normal Ax) �
     | inr hq => exact hqr hq;
   | _ => simp_all [valid_on_KripkeFrameClass, valid_on_KripkeFrame, valid_on_KripkeModel, kripke_satisfies];
 
-instance instSound [Ax.DefinesKripkeFrameClass 𝔽] : Sound (DeductionParameter.Normal Ax) 𝔽 := ⟨sound⟩
+instance instSound [Ax.DefinesKripkeFrameClass 𝔽] : Sound Axᴺ 𝔽 := ⟨sound⟩
 
 instance : Sound 𝐊 (AllFrameClass α) := by
   simpa [←Normal.isK] using (instSound (Ax := 𝗞) (𝔽 := AllFrameClass α));
 
-lemma unprovable_bot (𝔽 : FrameClass α) [Ax.DefinesKripkeFrameClass 𝔽] [nonempty : 𝔽.IsNonempty] : (Normal Ax) ⊬! ⊥ := by
+
+lemma unprovable_bot (𝔽 : FrameClass α) [Ax.DefinesKripkeFrameClass 𝔽] [nonempty : 𝔽.IsNonempty] : Axᴺ ⊬! ⊥ := by
   by_contra hC;
   obtain ⟨F, hF⟩ := nonempty.nonempty
   simpa using sound hC F hF;
 
-lemma consistent (𝔽 : FrameClass α) [Ax.DefinesKripkeFrameClass 𝔽] [𝔽.IsNonempty] : System.Consistent (Normal Ax) := by
+lemma consistent (𝔽 : FrameClass α) [Ax.DefinesKripkeFrameClass 𝔽] [𝔽.IsNonempty] : System.Consistent Axᴺ := by
   apply System.Consistent.of_unprovable;
   exact unprovable_bot 𝔽;
 
-private instance instConsistent_of_K' : System.Consistent ((Normal 𝗞) : DeductionParameter α) := consistent (𝔽 := AllFrameClass α)
+private instance instConsistent_of_K' : System.Consistent (𝗞ᴺ : DeductionParameter α) := consistent (𝔽 := AllFrameClass α)
 
 instance instConsistent_of_K : System.Consistent (𝐊 : DeductionParameter α) := by
   simpa [←Normal.isK] using instConsistent_of_K';
 
 
+
+lemma finite_sound [definability : Ax.DefinesFiniteKripkeFrameClass 𝔽] (d : Axᴺ ⊢! p) : 𝔽ᶠ ⊧ p := by
+  induction d using Deduction.inducition_with_necOnly! with
+  | hMaxm h =>
+    simp only [Set.mem_setOf_eq] at h;
+    rcases h with (hK | hR);
+    . exact (Semantics.RealizeSet.setOf_iff.mp valid_on_KripkeFrameClass.axiomK) _ hK;
+    . intro F hF;
+      simp [FrameClass.toFinite] at hF;
+      apply Semantics.RealizeSet.setOf_iff.mp (definability.defines hF.2 |>.mpr hF.1) _ hR;
+  | hMdp ihpq ihp => exact valid_on_KripkeFrameClass.mdp ihpq ihp;
+  | hNec ih => exact valid_on_KripkeFrameClass.nec ih;
+  | hDisj₃ =>
+    simp_all [valid_on_KripkeFrameClass, valid_on_KripkeFrame, valid_on_KripkeModel, kripke_satisfies];
+    intros; rename_i hpr hqr hpq;
+    cases hpq with
+    | inl hp => exact hpr hp;
+    | inr hq => exact hqr hq;
+  | _ => simp_all [valid_on_KripkeFrameClass, valid_on_KripkeFrame, valid_on_KripkeModel, kripke_satisfies];
+
+instance instFiniteSound [Ax.DefinesFiniteKripkeFrameClass 𝔽] : Sound Axᴺ 𝔽ᶠ := ⟨finite_sound⟩
+
+lemma unprovable_bot_finite (𝔽 : FrameClass α) [Ax.DefinesFiniteKripkeFrameClass 𝔽] [nonempty : 𝔽ᶠ.IsNonempty] : Axᴺ ⊬! ⊥ := by
+  by_contra hC;
+  obtain ⟨F, hF⟩ := nonempty.nonempty;
+  simpa using finite_sound hC F hF;
+
+lemma consistent_finite (𝔽 : FrameClass α) [Ax.DefinesFiniteKripkeFrameClass 𝔽] [𝔽ᶠ.IsNonempty] : System.Consistent Axᴺ := by
+  apply System.Consistent.of_unprovable;
+  exact unprovable_bot_finite 𝔽;
 
 end LO.Modal.Standard.Kripke
